Finish Lob's theorem (assuming the diagonal lemma)
Now working on the diagonal lemma, which hopefully won't be too much
more painful than Lob's theorem.  Admittedly, Lob's theorem was pretty
painful, with all the context munging that went on.  Hopefully, actually
instantiating that with the definitions of substitution and the like
will make things reduce definitionally.

internal/WellTypedLobsTheoremPreProof.v
@@ -3,86 +3,23 @@ Require Export Lob.Notations Lob.WellTypedLobsTheoremStatement.
 
 (** The proof of the theorem *)
 
+Axiom proof_admitted : False.
+Ltac admit' := case proof_admitted.
+
 Ltac do_shelve tac := tac; [ shelve | | ].
 
-Module Type TermPrimitives (Export LC : LobContext).
+Module Type TermPrimitives0 (Export LC : LobContext).
   Notation W := weakenTyp.
 
   Axiom weakenTerm : forall {Γ A B}, Term B -> Term (@weakenTyp Γ A B).
 
   Notation w := weakenTerm.
 
-  Axiom substTyp_weakenTyp
-  : forall {Γ A B a},
-      @Term Γ (@substTyp Γ A (@weakenTyp Γ A B) a) -> @Term Γ B.
-  Notation SW := substTyp_weakenTyp.
-
-  Axiom tProd : forall {Γ} A, Typ (Γ ▻ A) -> Typ Γ.
-  Definition tProd_nd : forall {Γ}, Typ Γ -> Typ Γ -> Typ Γ
-    := fun Γ A B => @tProd Γ A (W B).
-  Notation "A ‘→’ B" := (tProd A B) : typ_scope.
-  Notation "A ‘→'’ B" := (tProd_nd A B) : typ_scope.
-
-  Axiom tLambda : forall {Γ A B}, @Term (Γ ▻ A) B -> Term (A ‘→’ B).
-  Definition tLambda_nd : forall {Γ A B},
-                            @Term Γ B -> Term (A ‘→'’ B)
-    := fun Γ A B b => @tLambda Γ A (W B) (w b).
-  Notation "‘λ.’" := tLambda : term_scope.
-  Notation "‘λ'.’" := tLambda_nd : term_scope.
-
-  Axiom tApp : forall {Γ A B}
-                      (f : Term (@tProd Γ A B))
-                      (x : Term A),
-                 Term (B ‘’ x).
-  Definition tApp_nd : forall {Γ A B},
-                         Term (@tProd_nd Γ A B)
-                         -> Term A
-                         -> Term B
-    := fun Γ A B f x => SW (@tApp Γ A (W B) f x).
-  Notation "f ‘’ₐ x" := (tApp f x) : term_scope.
-  Notation "f ‘'’ₐ x" := (tApp_nd f x) : term_scope.
-
-  Axiom weakenTyp_tProd : forall {Γ A B C},
-                            Term (@weakenTyp Γ C (A ‘→'’ B))
-                            -> Term (@weakenTyp Γ C A ‘→’ W (W B)).
-  Definition weakenProd : forall {Γ A B C},
-                            Term (A ‘→'’ B)
-                            -> Term (@weakenTyp Γ C A ‘→’ W (W B))
-    := fun Γ A B C x => weakenTyp_tProd (w x).
-  Notation "w∀" := weakenProd.
-
-  (*Axiom weakenTyp1 : forall {Γ A B}, Typ (Γ ▻ B) -> Typ (Γ ▻ A ▻ (weakenTyp B)).
+  Axiom weakenTyp1 : forall {Γ A B}, Typ (Γ ▻ B) -> Typ (Γ ▻ A ▻ (weakenTyp B)).
+  Notation W1 := weakenTyp1.
 
   Axiom weakenTerm1 : forall {Γ A B C}, @Term (Γ ▻ B) C -> @Term (Γ ▻ A ▻ weakenTyp B) (@weakenTyp1 Γ A B C).
-
-  Axiom weakenTyp2 : forall {Γ A B C}, Typ (Γ ▻ B ▻ C) -> Typ (Γ ▻ A ▻ (weakenTyp B) ▻ (weakenTyp1 C)).
-
-  Axiom weakenTerm2 : forall {Γ A B C D}, Term D -> Term (@weakenTyp2 Γ A B C D).
-
-  Axiom weakenTyp3 : forall {Γ A B C D}, Typ (Γ ▻ B ▻ C ▻ D) -> Typ (Γ ▻ A ▻ (weakenTyp B) ▻ (weakenTyp1 C) ▻ (weakenTyp2 D)).
-
-  Axiom weakenTerm3 : forall {Γ A B C D E}, Term E -> Term (@weakenTyp3 Γ A B C D E).
-
-  Axiom weakenTyp4 : forall {Γ A B C D E}, Typ (Γ ▻ B ▻ C ▻ D ▻ E) -> Typ (Γ ▻ A ▻ (weakenTyp B) ▻ (weakenTyp1 C) ▻ (weakenTyp2 D) ▻ (weakenTyp3 E)).
-
-  Axiom weakenTerm4 : forall {Γ A B C D E F}, Term F -> Term (@weakenTyp4 Γ A B C D E F).
-
-  Axiom weakenTyp5 : forall {Γ A B C D E F}, Typ (Γ ▻ B ▻ C ▻ D ▻ E ▻ F) -> Typ (Γ ▻ A ▻ (weakenTyp B) ▻ (weakenTyp1 C) ▻ (weakenTyp2 D) ▻ (weakenTyp3 E) ▻ (weakenTyp4 F)).
-
-  Axiom weakenTerm5 : forall {Γ A B C D E F G}, Term G -> Term (@weakenTyp5 Γ A B C D E F G).
-
-  Notation W := weakenTyp (only parsing).
-  Notation W1 := weakenTyp1.
-  Notation W2 := weakenTyp2.
-  Notation W3 := weakenTyp3.
-  Notation W4 := weakenTyp4.
-  Notation W5 := weakenTyp5.
-  Notation w := weakenTerm.
   Notation w1 := weakenTerm1.
-  Notation w2 := weakenTerm2.
-  Notation w3 := weakenTerm3.
-  Notation w4 := weakenTerm4.
-  Notation w5 := weakenTerm5.
 
   Axiom substTerm1 : forall {Γ A B C}
                             (c : Term C)
@@ -95,7 +32,6 @@ Module Type TermPrimitives (Export LC : LobContext).
                            (a : Term A),
                       Typ (Γ ▻ substTyp B a ▻ substTyp1 C a).
   Notation "f ‘’₂ x" := (@substTyp2 _ _ _ _ f x) : typ_scope.
-
 
   Axiom substTerm2 : forall {Γ A B C D}
                             (c : Term D)
@@ -115,153 +51,204 @@ Module Type TermPrimitives (Export LC : LobContext).
                        Term (@substTyp3 Γ A B C D E a).
   Notation "f ‘’₃ x" := (@substTerm3 _ _ _ _ _ _ f x) : term_scope.
 
-  Axiom substTyp4 : forall {Γ A B C D E}
-                           (F : Typ (Γ ▻ A ▻ B ▻ C ▻ D ▻ E))
-                           (a : Term A),
-                      Typ (Γ ▻ substTyp B a ▻ substTyp1 C a ▻ substTyp2 D a ▻ substTyp3 E a).
-  Notation "f ‘’₄ x" := (@substTyp4 _ _ _ _ _ _ f x) : typ_scope.
+(*  Axiom W1W__to__WW : forall {Γ A B C},
+                        @Term (Γ ▻ A ▻ B) (W1 (W C))
+                        -> @Term (Γ ▻ A ▻ B) (W (W C)).*)
 
-  Axiom substTerm4 : forall {Γ A B C D E F}
-                            (f : Term F)
-                            (a : Term A),
-                       Term (@substTyp4 Γ A B C D E F a).
-  Notation "f ‘’₄ x" := (@substTerm4 _ _ _ _ _ _ _ f x) : term_scope.
+  Axiom substTyp_weakenTyp
+  : forall {Γ A B a},
+      @Term Γ (@substTyp Γ A (@weakenTyp Γ A B) a) -> @Term Γ B.
+  Notation SW := substTyp_weakenTyp.
 
-  Axiom subst_weaken1_weaken_Typ
-  : forall {Γ A B C a},
-      Term (@substTyp _ _ (@weakenTyp1 Γ C A (@weakenTyp Γ A B)) a) -> Term (@weakenTyp _ C B).
+  Axiom substTyp_weakenTyp1_weakenTyp
+  : forall {Γ T A B}
+           {a : Term (W B)},
+      @Term (Γ ▻ T) (W1 (W A) ‘’ a)
+      -> @Term (Γ ▻ T) (W A).
+  Notation SW1W := substTyp_weakenTyp1_weakenTyp.
 
-  Axiom Subst1_Subst_Weaken_Weaken
-  : forall {Γ C B A a b},
-      @Term Γ ((A ‘→’ B ‘→’ C) ‘’₁ a ‘’ b)
-      -> @Term Γ C.
+  Axiom substTyp1_substTyp_weakenTyp_inv
+  : forall {Γ C T A} {a : @Term Γ C} {b : @Term Γ (T ‘’ a)},
+      @Term Γ (A ‘’ a)
+      -> @Term Γ (@weakenTyp _ _ A ‘’₁ a ‘’ b).
 
-  Axiom subst_Weaken1__weaken_Typ
-  : forall {Γ T B A a},
-      @Term (Γ ▻ T) (W (A ‘’ a))
-      -> @Term (Γ ▻ T) (@weakenTyp1 _ _ _ A ‘’ @weakenTerm _ _ B a).
+  Notation S₁₀W' := substTyp1_substTyp_weakenTyp_inv.
 
-  Notation W1w := subst_Weaken1__weaken_Typ.
+  (*Axiom substTyp2_substTyp1_substTyp_weakenTyp1_weakenTyp1_inv
+  : forall {Γ A B C}
+           {a : @Term Γ A}
+           {T : Typ (Γ ▻ C)}
+           {b : @Term Γ (B ‘’ a)}
+           {c : @Term Γ (W C ‘’ a)},
+      @Term Γ (T ‘’ SW c)
+      -> @Term Γ (W1 (W1 T) ‘’₂ a ‘’₁ b ‘’ S₁₀W' c).
 
-  Axiom Subst_Subst1_Weaken2__weaken__W1w
-  : forall {Γ B C T A a b},
-      @Term (Γ ▻ T) (W (A ‘’₁ a ‘’ b))
-      -> @Term (Γ ▻ T) (@weakenTyp2 _ _ B _ A ‘’₁ w a ‘’ W1w (A := C) (w b)).
+  Notation S₂₁₀W1W1' := substTyp2_substTyp1_substTyp_weakenTyp1_weakenTyp1_inv.*)
 
-  Axiom Subst_Subst1_Subst_Weaken1_Weaken1
-  : forall {Γ} {B C : Typ Γ} {D : Typ (Γ ▻ B)}
-           {A : Typ (Γ ▻ C)}
-           {a : @Term (Γ ▻ B ▻ D) (D ‘→’ B ‘→’ C)}
+  Axiom substTyp2_substTyp1_substTyp_weakenTyp_weakenTyp_inv
+  : forall {Γ B}
            {b : @Term Γ B}
-           {c : @Term Γ (D ‘’ b)},
-      @Term Γ (A ‘’ (Subst1_Subst_Weaken_Weaken (a ‘’₁ b ‘’ c)))
-      -> @Term Γ (W1 (A := D) (W1 (A := B) (B := C) A) ‘’ a ‘’₁ b ‘’ c).
+           {C D}
+           {A : Typ (Γ ▻ B)}
+           {c : @Term Γ (C ‘’ b)}
+           {d : @Term Γ (D ‘’₁ b ‘’ c)},
+      @Term Γ (W (W A) ‘’₂ b ‘’₁ c ‘’ d)
+      -> @Term Γ (A ‘’ b).
 
-  Axiom Subst_Subst2__Weaken3_Subst2__Subst1_Weaken2_Weaken2__weaken__W1w_w__SS1W2wW1w_w_SS1SW1W1
-  : forall {Γ}
-           {T D : Typ Γ}
-           {E : Typ (Γ ▻ D)}
-           {B : Typ Γ}
-           {C : Typ (Γ ▻ B)}
-           {A : Typ (Γ ▻ B ▻ C)}
-           {a : Term (E ‘→’ D ‘→’ B)}
-           {b : Term D}
-           {c : Term (E ‘’ b)}
-           {d : Term (C ‘’ Subst1_Subst_Weaken_Weaken (a ‘’₁ b ‘’ c))},
-      @Term (Γ ▻ T) (W (A ‘’₁ (Subst1_Subst_Weaken_Weaken (a ‘’₁ b ‘’ c)) ‘’ d))
-      -> @Term (Γ ▻ T) (W3 (B := D) (C := E) (W2 (W2 (B := B) (C := C) A) ‘’₁ a) ‘’₂ w b ‘’₁ W1w (w c) ‘’ Subst_Subst1_Weaken2__weaken__W1w
-                        (w (Subst_Subst1_Subst_Weaken1_Weaken1 d))).
-*)
-  (*Axiom subst_weaken1_weaken_Typ_inv
-  : forall {Γ A B C a},
-      Term (@weakenTyp _ C B) -> Term (@substTyp _ _ (@weakenTyp1 Γ C A (@weakenTyp Γ A B)) a).*)
+  Notation S₂₁₀WW' := substTyp2_substTyp1_substTyp_weakenTyp_weakenTyp_inv.
 
-(*Check ‘Term’%typ.
-  Definition subst_weaken_many_Typ_0
-  : forall {Γ A B C D E F G} {Z : Typ (Γ ▻ A ▻ B)} {Y} {a b c d e},
-      Term (substTyp1
-              (substTyp2
-                 (substTyp3
-                    (substTyp4
-                       (@weakenTyp5 _ G _ _ _ _ _ (@weakenTyp1 _ F _ (@weakenTyp1 _ E _ (@weakenTyp1 _ D _ (@weakenTyp1 _ C _ Z)) ‘’ Y))) a) b) c) d ‘’ e)
-      -> Type.
-Arguments Term : clear implicits.
-intros.
-refine (@Term (Γ ▻ G) _).
-refine (substTyp (substTyp1 (W2 Z) a) (_ (substTerm (substTerm1 (substTerm2 (substTerm3 (substTerm4 (w5 (w1 Y)) a) b) c) d) e))); shelve_unifiable.
-pose @subst_weaken1_weaken_Typ.
+  Axiom weakenTyp_substTyp_substTyp2_substTyp1_substTyp_weakenTyp1_weakenTyp1_inv
+  : forall {Γ T' B C D A}
+           {a : @Term (Γ ▻ B ▻ C ▻ W D) (W (W A))}
+           {T : Typ (Γ ▻ B ▻ A)}
+           {b : @Term Γ B}
+           {c : @Term Γ (C ‘’ b)}
+           {d : @Term Γ (D ‘’ b)},
+      @Term (Γ ▻ T') (W (T ‘’₁ b ‘’ (S₂₁₀WW' (a ‘’₂ b ‘’₁ c ‘’ S₁₀W' d))))
+      -> @Term (Γ ▻ T') (W ((W1 (W1 T)) ‘’ a ‘’₂ b ‘’₁ c ‘’ S₁₀W' d)).
 
-      -> Term (substTyp1
-              (substTyp2
-                 (substTyp3
-                    (substTyp4
-                       (@weakenTyp5 _ G _ _ _ _ _ (@weakenTyp1 _ F _ (@weakenTyp1 _ E _ (@weakenTyp1 _ D _ (@weakenTyp1 _ C _ Z)) ‘’ Y))) a) b) c) d ‘’ e).
- "Term (ε ▻ ?A0)
-    (substTyp1
-       (substTyp2
-          (substTyp3
-             (substTyp4 (W5 (W1 (W1 (W1 (W1 ‘Term’)) ‘’ qsubstTyp))) ?t3)
-             ?t) ?t0) f ‘’ x)" while it is expected to have type
- "Term (ε ▻ ?A0) (?A0 ‘→’ ‘□’ ‘’ ⌜ ‘X’ ⌝%typ)".
-_*)
+  Notation WS₀₂₁₀W1W1' := weakenTyp_substTyp_substTyp2_substTyp1_substTyp_weakenTyp1_weakenTyp1_inv.
 
-End TermPrimitives.
+  Axiom weakenTyp_substTyp2_substTyp1_substTyp_weakenTyp_inv
+  : forall {Γ A B C T T'}
+           {a : @Term Γ A}
+           {b : @Term Γ (B ‘’ a)}
+           {c : @Term Γ (C ‘’₁ a ‘’ b)},
+      @Term (Γ ▻ T') (W (T ‘’₁ a ‘’ b))
+      -> @Term (Γ ▻ T') (W (W T ‘’₂ a ‘’₁ b ‘’ c)).
 
-Module Type QuotedPrimitives (Export LC : LobContext) (Export TP : TermPrimitives LC).
-  Axiom qcontext_extend : □ (‘Context’ ‘→’ ‘Typ’ ‘→'’ W ‘Context’).
-  Notation "Γ ‘▻’ x" := (qcontext_extend ‘’ₐ Γ ‘'’ₐ x)%term : term_scope.
-  Notation "Γ ‘▻’ x" := (Γ ‘▻’ x)%term : context_scope.
+  Notation WS₂₁₀W' := weakenTyp_substTyp2_substTyp1_substTyp_weakenTyp_inv.
 
-  (*Axiom VAR1 : forall {Γ A B}, @Term (Γ ▻ A ▻ B) (weakenTyp (weakenTyp A)).
-  Notation "‘VAR₁’" := VAR1 : term_scope.*)
+  Axiom substTyp3_substTyp2_substTyp1_substTyp_weakenTyp
+  : forall {Γ A B C D T T'}
+           {a : @Term Γ A}
+           {b : @Term Γ (B ‘’ a)}
+           {c : @Term Γ (C ‘’₁ a ‘’ b)}
+           {d : @Term (Γ ▻ T') (W (D ‘’₂ a ‘’₁ b ‘’ c))},
+      @Term (Γ ▻ T') (W1 (W T ‘’₃ a ‘’₂ b ‘’₁ c) ‘’ d)
+      -> @Term (Γ ▻ T') (W (T ‘’₂ a ‘’₁ b ‘’ c)).
 
-  (*Axiom qsubstTyp : @Term (ε ▻ ‘Context’ ▻ ‘Typ’ ▻ (W1 (W1 ‘Typ’) ‘’ qcontext_extend) ▻ W ‘Term’) (W (W (W ‘Typ’))).
-  Notation "f ‘‘’’ x" := (substTerm (substTerm1 (substTerm2 (substTerm3 qsubstTyp _) _) f) x) : typ_scope.
-  Axiom qsubstTerm : @Term (ε ▻ ‘Context’ ▻ ‘Typ’ ▻ (W1 (W1 ‘Typ’) ‘’ qcontext_extend) ▻ substTyp1 (W2 (W2 ‘Term’)) _ ▻ W (W ‘Term’))
-                           (W1 (W1 (W1 (W1 ‘Term’)) ‘’ qsubstTyp)).
-  Notation "f ‘‘’’ x" := (substTerm (substTerm1 (substTerm2 (substTerm3 (substTerm4 qsubstTerm _) _) _) f) x) : term_scope.
+  Notation W1S₃₂₁₀W := substTyp3_substTyp2_substTyp1_substTyp_weakenTyp.
 
-  (** XXX Is this actually true? *)
-  Axiom Conv0_Typ
-  : forall {qH0},
-      □ (‘Typ’ ‘’ ⌜ ε ▻ ‘Term’ ‘’₁ ⌜ ε ⌝%ctx ‘’ qH0 ⌝%ctx)
-      -> □ (‘Typ’ ‘’ (‘ε’ ‘▻’ qH0)%ctx).
-  Axiom Conv0_Term
-  : forall {T qH0 qH0'},
-      Term (T ‘→’ ‘Term’ ‘’₁ ⌜ ε ▻ ‘Term’ ‘’₁ ⌜ ε ⌝%ctx ‘’ qH0 ⌝%ctx ‘’ qH0') ->
-      Term (T ‘→’ ‘Term’ ‘’₁ (‘ε’ ‘▻’ qH0)%ctx ‘’ Conv0_Typ qH0').
+  Axiom weakenTyp_substTyp2_substTyp1_substTyp_weakenTyp1
+  : forall {Γ A B C T T'}
+           {a : @Term Γ A}
+           {b : Term (B ‘’ a)}
+           {c : Term (C ‘’ a)},
+      @Term (Γ ▻ T') (W (W1 T ‘’₂ a ‘’₁ b ‘’ S₁₀W' c))
+      -> @Term (Γ ▻ T') (W (T ‘’₁ a ‘’ c)).
 
-  Axiom qquote_context : @Term (ε ▻ ‘Context’) (W ((substTyp1 ‘Term’ ‘ε’) ‘’ ⌜ ‘Context’ ⌝%typ)).*)
+  Notation WS₂₁₀W1 := weakenTyp_substTyp2_substTyp1_substTyp_weakenTyp1.
 
-(*
-  Definition qqempty_context := qquote_context ε.
-  Notation "‘ε’" := qempty_context : term_scope.
-  Notation "⌜ x ⌝" := (quote_context x) : context_scope.
 
-  Axiom qTerm : Typ (ε ▻ ‘Context’ ▻ ‘Typ’).
-  Notation "‘Term’" := qTerm : typ_scope.
+  Axiom tProd : forall {Γ} A, Typ (Γ ▻ A) -> Typ Γ.
+  Definition tProd_nd : forall {Γ}, Typ Γ -> Typ Γ -> Typ Γ
+    := fun Γ A B => @tProd Γ A (W B).
+  Notation "A ‘→’ B" := (tProd A B) : typ_scope.
+  Notation "A ‘→'’ B" := (tProd_nd A B) : typ_scope.
 
-  Definition qbox := (substTyp1 ‘Term’ ‘ε’).
-  Notation "‘□’" := qbox : typ_scope.
+  Axiom tLambda : forall {Γ A B}, @Term (Γ ▻ A) B -> Term (A ‘→’ B).
+  Definition tLambda_nd : forall {Γ A B},
+                            @Term Γ B -> Term (A ‘→'’ B)
+    := fun Γ A B b => @tLambda Γ A (W B) (w b).
+  Notation "‘λ.’" := tLambda : term_scope.
+  Notation "‘λ'.’" := tLambda_nd : term_scope.
 
-  Axiom quote_typ : forall {Γ}, Typ Γ -> □ (‘Typ’ ‘’ ⌜ Γ ⌝%ctx).
-  Notation "⌜ x ⌝" := (quote_typ x%typ) : typ_scope.
-  Axiom quote_term : forall {Γ} {A : Typ Γ}, Term A -> □ ((substTyp1 ‘Term’ ⌜ Γ ⌝%ctx) ‘’ ⌜ A ⌝%typ).
-  Notation "⌜ x ⌝" := (quote_term x%term) : term_scope.
+  Axiom substTyp_tProd : forall {Γ T A B a},
+                           Term (@tProd (Γ ▻ T) A B ‘’ a)
+                           -> Term (@tProd Γ (A ‘’ a) (B ‘’₁ a)).
+  Notation "S∀" := substTyp_tProd.
 
-  Notation "x ‘→’ y" := (@weakenTyp _ x%typ y) : typ_scope.
-*)
-  (*Axiom qsubstTyp : @Term (ε ▻ ‘Context’ ▻ ‘Typ’ ▻ (W1 (W1 ‘Typ’) ‘’ qcontext_extend) ▻ W ‘Term’) (W (W (W ‘Typ’))).
+  Axiom substTyp1_substTyp_tProd
+  : forall {Γ T T' A B a b},
+      Term (@tProd (Γ ▻ T ▻ T') A B ‘’₁ a ‘’ b)
+      -> Term (@tProd Γ (A ‘’₁ a ‘’ b) (B ‘’₂ a ‘’₁ b)).
+  Notation "S₁₀∀" := substTyp1_substTyp_tProd.
 
-  Axiom qweakenTyp : forall {Γ A}, Typ Γ -> Typ (Γ ▻ A).
-  Axiom substTyp1 : forall {Γ A B}
-                           (C : Typ (Γ ▻ A ▻ B))
-                           (a : Term A),
-                      Typ (Γ ▻ substTyp B a).*)
+  Axiom substTyp2_substTyp1_substTyp_tProd
+  : forall {Γ T T' T'' A B a b c},
+      Term (@tProd (Γ ▻ T ▻ T' ▻ T'') A B ‘’₂ a ‘’₁ b ‘’ c)
+      -> Term (@tProd Γ (A ‘’₂ a ‘’₁ b ‘’ c) (B ‘’₃ a ‘’₂ b ‘’₁ c)).
+  Notation "S₂₁₀∀" := substTyp2_substTyp1_substTyp_tProd.
 
-End QuotedPrimitives.
+  Axiom weakenTyp_substTyp2_substTyp1_substTyp_tProd
+  : forall {Γ T T' T'' T''' A B a b c},
+      Term (@weakenTyp _ T''' (@tProd (Γ ▻ T ▻ T' ▻ T'') A B ‘’₂ a ‘’₁ b ‘’ c))
+      -> Term (@tProd (Γ ▻ T''') (W (A ‘’₂ a ‘’₁ b ‘’ c)) (W1 (B ‘’₃ a ‘’₂ b ‘’₁ c))).
+  Notation "WS₂₁₀∀" := weakenTyp_substTyp2_substTyp1_substTyp_tProd.
 
-Module Type TypeQuine (Export LC : LobContext) (Export LH : LobHypotheses LC) (Export TP : TermPrimitives LC).
+
+  Axiom tApp : forall {Γ A B}
+                      (f : Term (@tProd Γ A B))
+                      (x : Term A),
+                 Term (B ‘’ x).
+  Definition tApp_nd : forall {Γ A B},
+                         Term (@tProd_nd Γ A B)
+                         -> Term A
+                         -> Term B
+    := fun Γ A B f x => SW (@tApp Γ A (W B) f x).
+  Notation "f ‘’ₐ x" := (tApp f x) : term_scope.
+  Notation "f ‘'’ₐ x" := (tApp_nd f x) : term_scope.
+
+  Axiom weakenTyp_tProd_nd : forall {Γ A B C},
+                            Term (@weakenTyp Γ C (A ‘→'’ B))
+                            -> Term (@weakenTyp Γ C A ‘→'’ W B).
+  Definition weakenProd_nd : forall {Γ A B C},
+                               Term (A ‘→'’ B)
+                               -> Term (@weakenTyp Γ C A ‘→'’ W B)
+    := fun Γ A B C x => weakenTyp_tProd_nd (w x).
+  Notation "w→" := weakenProd_nd.
+
+  Axiom weakenTyp_tProd : forall {Γ A B C},
+                            Term (@weakenTyp Γ C (A ‘→’ B))
+                            -> Term (@weakenTyp Γ C A ‘→’ W1 B).
+  Definition weakenProd : forall {Γ A B C},
+                            Term (A ‘→’ B)
+                            -> Term (@weakenTyp Γ C A ‘→’ W1 B)
+    := fun Γ A B C x => weakenTyp_tProd (w x).
+  Notation "w∀" := weakenProd.
+
+  Axiom weakenTyp_tProd_tProd_nd
+  : forall {Γ A B C D},
+      Term (@weakenTyp Γ D (A ‘→’ B ‘→'’ C))
+      -> Term (@weakenTyp Γ D A ‘→’ W1 B ‘→'’ W1 C).
+  Definition weakenProd_Prod_nd
+  : forall {Γ A B C D},
+      Term (A ‘→’ B ‘→'’ C)
+      -> Term (@weakenTyp Γ D A ‘→’ W1 B ‘→'’ W1 C)
+    := fun Γ A B C D x => weakenTyp_tProd_tProd_nd (w x).
+  Notation "w∀→" := weakenProd_Prod_nd.
+End TermPrimitives0.
+
+Module Type QuotedPrimitives0 (Export LC : LobContext) (Export TP0 : TermPrimitives0 LC).
+  Axiom qtProd_nd
+  : @Term (ε ▻ ‘Context’ ▻ ‘Typ’ ▻ W ‘Typ’) (W (W ‘Typ’)).
+  Notation "‘tProd_nd’" := qtProd_nd.
+
+  Axiom qtApp_nd
+  : □ (‘Context’ ‘→’ ‘Typ’ ‘→’ W ‘Typ’
+        ‘→’ W1 (W1 ‘Term’) ‘’ ‘tProd_nd’
+        ‘→'’ W ‘Term’
+        ‘→'’ W1 ‘Term’).
+  Notation "‘tApp_nd’" := qtApp_nd.
+
+  (* XXX Is this actually true? *)
+  Axiom Conv0
+  : forall {qH0 qX},
+      @Term (ε ▻ ‘Term’ ‘’₁ ‘ε’ ‘’ qH0)
+            (W (‘Term’ ‘’₁ ‘ε’ ‘’ ⌜ ‘Term’ ‘’₁ ‘ε’ ‘’ qH0 ‘→'’ qX ⌝%typ))
+      -> @Term (ε ▻ ‘Term’ ‘’₁ ‘ε’ ‘’ qH0)
+               (W
+                  (‘Term’ ‘’₁ ‘ε’
+                    ‘’ S₂₁₀WW' (‘tProd_nd’ ‘’₂ ‘ε’ ‘’₁ ⌜ ‘Term’ ‘’₁ ‘ε’ ‘’ qH0 ⌝%typ ‘’ S₁₀W' ⌜ qX ⌝%typ))).
+
+  Axiom qquote_term : forall {A : Typ ε},
+                        @Term ε (A ‘→'’ ‘Term’ ‘’₁ _ ‘’ ⌜ A ⌝%typ).
+  Notation "‘quote_term’" := qquote_term : term_scope.
+
+End QuotedPrimitives0.
+
+Module Type TypeQuine (Export LC : LobContext) (Export LH : LobHypotheses LC) (Export TP0 : TermPrimitives0 LC).
   Axiom H0 : Typ ε.
   Definition H := Term H0.
   Definition qH0 := quote_typ H0.
@@ -280,533 +267,106 @@ Module Type TypeQuine (Export LC : LobContext) (Export LH : LobHypotheses LC) (E
   Notation "‘fromH’" := qfromH : term_scope.
 End TypeQuine.
 
-Module Lob1'
+Module Lob0
+       (LC : LobContext)
+       (LH : LobHypotheses LC)
+       (Export TP0 : TermPrimitives0 LC)
+       (Export QP0 : QuotedPrimitives0 LC TP0)
+       (Export TQ : TypeQuine LC LH TP0)
+<: LobsTheorem LC LH.
+
+  Definition lob : X.
+  Proof.
+    refine (let h : H := toH
+                           (‘λ.’
+                              ((w→ (‘λ.’ ‘f’))
+                                 ‘'’ₐ _))%term in
+            f (fromH h ‘'’ₐ ⌜ h ⌝)%term); shelve_unifiable.
+    refine (let f := Conv0 (SW1W (w∀ ‘fromH’ ‘’ₐ ‘VAR₀’)) in
+            let x := (w→ ‘quote_term’ ‘'’ₐ ‘VAR₀’)%term in
+            WS₂₁₀W1
+              (W1S₃₂₁₀W
+                 (WS₂₁₀∀
+                      (W1S₃₂₁₀W
+                         (w∀ (S₂₁₀∀ (S₁₀∀ (S∀ (‘tApp_nd’ ‘’ₐ ‘ε’) ‘’ₐ ⌜ ‘H’ ⌝%typ) ‘’ₐ S₁₀W' ⌜ ‘X’ ⌝%typ))
+                             ‘’ₐ WS₀₂₁₀W1W1' f))
+                      ‘’ₐ WS₂₁₀W' x))%term).
+  Defined.
+End Lob0.
+
+Module Type TermPrimitives (Export LC : LobContext).
+  Include (TermPrimitives0 LC).
+
+  Axiom context_eq_dec : forall Γ Γ' : Context, {Γ = Γ'} + {Γ <> Γ'}.
+  Axiom context_eq_dec_refl : forall Γ, context_eq_dec Γ Γ = left eq_refl.
+
+  Axiom qsigT : forall (T : Typ ε), Typ (ε ▻ T) -> Typ ε.
+  Notation "‘sigT’" := qsigT.
+End TermPrimitives.
+
+Module Type QuotedPrimitives (Export LC : LobContext) (Export TP : TermPrimitives LC).
+  Include (QuotedPrimitives0 LC TP).
+
+  Axiom qcontext_extend : @Term (ε ▻ ‘Context’ ▻ ‘Typ’) (W (W ‘Context’)).
+  Notation "Γ ‘▻’ x" := (qcontext_extend ‘’₁ Γ ‘’ x)%typ : term_scope.
+  Notation "Γ ‘▻’ x" := (Γ ‘▻’ x)%term : context_scope.
+
+End QuotedPrimitives.
+
+Module TQ (Export LC : LobContext) (Export LH : LobHypotheses LC) (Export TP : TermPrimitives LC) (Export QP : QuotedPrimitives LC TP)
+<: TypeQuine LC LH TP.
+
+  Definition dummy : Typ ε := qContext.
+
+  Definition quote_sigma (Γv : { Γ : _ & Typ Γ }) : Term (‘sigT’ ‘Context’ ‘Typ’).
+  Proof.
+  Admitted.
+
+  Definition cast (Γv : { Γ : _ & Typ Γ }) : Typ (ε ▻ ‘sigT’ ‘Context’ ‘Typ’).
+  Proof.
+    refine (if context_eq_dec Γv.1 (ε ▻ ‘sigT’ ‘Context’ ‘Typ’)
+            then @eq_rect _ _ Typ Γv.2 _ _
+            else W dummy);
+      assumption.
+  Defined.
+
+  Definition H0 : Typ ε.
+  Proof.
+    refine (let h : { Γ : _ & Typ Γ }
+                := ((ε ▻ ‘sigT’ ‘Context’ ‘Typ’)%ctx;
+                    _ (W (‘Term’ ‘’₁ ‘ε’))%typ)
+            in (cast h ‘’ quote_sigma h ‘→'’ ‘X’)%typ).
+    admit'.
+  Defined.
+
+  Definition H := Term H0.
+  Definition qH0 := quote_typ H0.
+  Definition qH := ((substTyp1 ‘Term’ _) ‘’ qH0)%typ.
+  Notation "‘H’" := qH : typ_scope.
+  Definition H0' := (‘H’ ‘→'’ ‘X’)%typ.
+  Definition H' := Term H0'.
+  Definition qH0' := quote_typ H0'.
+  Definition qH' := ((substTyp1 ‘Term’ _) ‘’ qH0')%typ.
+  Notation "‘H'’" := qH' : typ_scope.
+
+  Definition toH : H' -> H.
+  Proof.
+    unfold H', H, H0, H0', qH, cast; simpl.
+    rewrite context_eq_dec_refl; simpl.
+
+  Axiom fromH : H -> H'.
+  Axiom qtoH : Term (‘H'’ ‘→'’ ‘H’).
+  Axiom qfromH : Term (‘H’ ‘→'’ ‘H'’).
+  Notation "‘toH’" := qtoH : term_scope.
+  Notation "‘fromH’" := qfromH : term_scope.
+End TQ.
+
+Module Lob
        (LC : LobContext)
        (LH : LobHypotheses LC)
        (Export TP : TermPrimitives LC)
        (Export QP : QuotedPrimitives LC TP)
-       (Export TQ : TypeQuine LC LH TP)
 <: LobsTheorem LC LH.
-  (*Notation "f ‘‘’’₅ x" := ((w5 qsubstTerm) ‘’₄ _ ‘’₃ _ ‘’₂ _ ‘’₁ f ‘’ x)%term : term_scope.*)
-
-  Definition lob : X.
-  Proof.
-Arguments Term : clear implicits.
-    refine (let h : H := toH
-                           (‘λ.’
-                              ((w∀ (‘λ.’ ‘f’))
-                                 ‘'’ₐ _))%term(*(subst_weaken1_weaken_Typ
-                                ((w1 ‘f’)
-                                   ‘’ (let f := Subst_Subst2__Weaken3_Subst2__Subst1_Weaken2_Weaken2__weaken__W1w_w__SS1W2wW1w_w_SS1SW1W1 (Conv0_Term ‘fromH’%term) : @Term (ε ▻ ‘H’) _ in
-                                       let x := _ in
-                                       (_ (f ‘‘’’₅ x)%term))))*) in
-            f (fromH h ‘'’ₐ ⌜ h ⌝)%term); shelve_unifiable.
-
-    refine (let k := (w∀ (tLambda ‘f’))%term in _); shelve_unifiable.
-    unfold tProd_nd.
-    unfold H'.
-    unfold H0'.
-     subst f.
-refine (let k := (W4 (W2 (W2 ‘Term’) ‘’₁ qcontext_extend
-            ‘→’ W1 (W1 ‘Typ’) ‘’ qcontext_extend ‘→’ ‘Term’) ‘’₃
-                                                            w ‘ε’ )%typ in _); shelve_unifiable.
-refine (let k' := (W3 ((W2 (W2 ‘Term’) ‘’₁ qcontext_extend
-            ‘→’ W1 (W1 ‘Typ’) ‘’ qcontext_extend ‘→’ ‘Term’) ‘’₃
-                                                           ‘ε’))%typ in _); shelve_unifiable.
-pose ((W2 (W2 ‘Term’) ‘’₁ qcontext_extend
-            ‘→’ W1 (W1 ‘Typ’) ‘’ qcontext_extend ‘→’ ‘Term’) ‘’₃
-                                                             ‘ε’)%typ.
-pose ((W2 (W2 ‘Term’) ‘’₁ qcontext_extend
-            ‘→’ W1 (W1 ‘Typ’) ‘’ qcontext_extend ‘→’ ‘Term’) ‘’₃
-                                                             ‘ε’)%typ.
-(W4
-           (W2 (W2 ‘Term’) ‘’₁ qcontext_extend
-            ‘→’ W1 (W1 ‘Typ’) ‘’ qcontext_extend ‘→’ ‘Term’) ‘’₃
-         w ‘ε’ ‘’₂ W1w (w qH0)
-         ‘’₁ Subst_Subst1_Weaken2__weaken__W1w
-               (w (Subst_Subst1_Subst_Weaken1_Weaken1 (Conv0_Typ qH0')))
-         ‘’ Subst_Subst2__Weaken3_Subst2__Subst1_Weaken2_Weaken2__weaken__W1w_w__SS1W2wW1w_w_SS1SW1W1
-              (Conv0_Term ‘fromH’))
-
-(W4
-           (W2 (W2 ‘Term’) ‘’₁ qcontext_extend
-            ‘→’ W1 (W1 ‘Typ’) ‘’ qcontext_extend ‘→’ ‘Term’) ‘’₃
-         w ‘ε’ ‘’₂ W1w (w qH0)
-         ‘’₁ Subst_Subst1_Weaken2__weaken__W1w
-               (w (Subst_Subst1_Subst_Weaken1_Weaken1 (Conv0_Typ qH0')))
-         ‘’ Subst_Subst2__Weaken3_Subst2__Subst1_Weaken2_Weaken2__weaken__W1w_w__SS1W2wW1w_w_SS1SW1W1
-              (Conv0_Term ‘fromH’))
-    unfold qH' in *.
-    pose qH0'.
-    unfold qH in *.
-    move t0 at top.
-    pose ‘H'’%typ.
-    unfold qH'.
-    unfold qH in *.
-    Unshelve
-
-match eval unfold t in t with
-  | ?f ?x => pose x
-end.
-pose (?t16@{x:=‘fromH’%term}).
-let t := type of ?t16 in assert t.
-unify ?t16 qH0'.
-
-Arguments Term : clear implicits.
-refine (let f := _ in
-        let x := _ in
-        let k := (substTerm (substTerm1 (substTerm2 (substTerm3 (substTerm4 (w5 qsubstTerm) _) _) _) f) x) in _); shelve_unifiable.
-unfold qH.
-
-(substTerm (substTerm1 (substTerm2 (substTerm3 (substTerm4 qsubstTerm _) _) _) f) x)
-
-
-    Set Printing Implicit.
-    unfold H', qH'.
-
-  Axiom qLetIn : forall {Γ A B}, Term (
-
-    Set Printing All.
-
-
-, Typ (Γ ▻ A) -> Term A -> Typ Γ.
-  Notation "f ‘’ x" := (@substTyp _ _ f x) : typ_scope.
-  Axiom weakenTyp : forall {Γ A}, Typ Γ -> Typ (Γ ▻ A).
-  Axiom substTerm : forall {Γ A} {B : Typ (Γ ▻ A)}
-
-
-    Focus 2.
-
-
-    refine ((fun (ℓ : □ L) => f (App (Conv2 ℓ) (Conv (Quot ℓ))))
-              (Conv2_inv
-                 (wttLambda_nd
-                    (‘□’ ‘’ ‘L’)
-                    (‘‘f’’ ‘’ ((‘‘App’’ ‘’ (qConv2 ‘‘VAR₀’’)) ‘’ ((*‘‘Conv’’ ‘’*) (‘‘Quote’’ ‘’ ‘‘VAR₀’’)))))));
-    try exact _.
-  Defined.
-End Lob1'.
-
-
-Module Type PretermPrimitives (Export LC : LobContext).
-  Axiom tLambda : Preterm -> Preterm -> Preterm.
-  Axiom qtApp : Preterm.
-
-  Notation "‘App’" := qtApp : preterm_scope.
-
-  Axiom qtProd : Preterm -> Preterm -> Preterm.
-  Notation "x ‘‘→’’ y" := (qtProd x y) : preterm_scope.
-
-  Axiom ttVar0 : forall {Γ T}, box' (Γ ▻ T) T.
-  Notation "‘‘VAR₀’’" := ttVar0 : well_typed_term_scope.
-
-  Axiom tVar0 : Preterm.
-  Notation "‘VAR₀’" := tVar0.
-
-End PretermPrimitives.
-
-Module Type PreL (LC : LobContext) (Export PP : PretermPrimitives LC).
-
-  Axiom wttLambda_nd : forall {Γ : Context} {B' : Preterm},
-                       forall A' : Preterm, box' (Γ ▻ A') B' -> box' Γ (A' ‘→’ B').
-
-  Axiom wttApp_1_nd : forall {Γ : Context} {A' B' : Preterm} {H : is_closed B'},
-                        box' Γ (A' ‘→’ B') -> box' Γ A' -> box' Γ B'.
-
-  Notation "x ‘’ y" := (wttApp_1_nd x%wtt y%wtt) : well_typed_term_scope.
-
-  (*Axiom box'_weaken : forall {Γ A}, box' ε A -> box' Γ A.*)
-End PreL.
-
-Module Lob1 (LC : LobContext) (Import LH : LobHypotheses LC).
-
-  Module Type PretermPrimitives' := PretermPrimitives LC.
-
-  Module Type L (PP : PretermPrimitives') (Export PL : PreL LC PP).
-    Axiom L : Preterm.
-    Axiom qL : Preterm.
-    Notation "‘L’" := qL.
-  End L.
-
-  Module Type PostL (PP : PretermPrimitives') (PL : PreL LC PP) (Export L' : L PP PL).
-    Axiom App : let A' := ‘□’ ‘’ ‘L’ in
-                let B' := ‘X’ in
-                □ (A' ‘→’ B') -> □ A' -> □ B'.
-
-    Axiom Conv : □ (‘□’ ‘’ ⌜ L ⌝) -> □ (‘□’ ‘’ ‘L’).
-
-    Axiom Conv2 : □ L -> □ (‘□’ ‘’ ‘L’ ‘→’ ‘X’).
-    Axiom Conv2_inv : □ (‘□’ ‘’ ‘L’ ‘→’ ‘X’) -> □ L.
-    Axiom qConv2 : let Γ := (ε ▻ ‘□’ ‘’ ‘L’) in
-                   box' Γ (‘□’ ‘’ ‘L’) -> box' Γ (‘□’ ‘’ (⌜ (‘□’ ‘’ ‘L’) ⌝ ‘‘→’’ ⌜ ‘X’ ⌝)).
-
-    Axiom Quot : □ L -> □ (‘□’ ‘’ ⌜ L ⌝).
-
-    Axiom qbApp
-    : let Γ := (ε ▻ ‘□’ ‘’ ‘L’) in
-      forall (A' := (⌜ ‘□’ ‘’ ‘L’ ⌝)%preterm)
-             (B' := (⌜ ‘X’ ⌝)%preterm),
-        box' Γ ((‘□’ ‘’ (A' ‘‘→’’ B')) ‘→’ ‘□’ ‘’ A' ‘→’ ‘□’ ‘’ B').
-
-    Notation "‘‘App’’" := ((*box'_weaken*) qbApp) : well_typed_term_scope.
-
-    (*Axiom qConv
-  : □ (‘□’ ‘’ ⌜‘□’ ‘’ ⌜L ⌝ ⌝ ‘→’ ‘□’ ‘’ ⌜ ‘□’ ‘’ ‘L’ ⌝).
-
-  Notation "‘‘Conv’’" := (box'_weaken qConv) : well_typed_term_scope.*)
-
-    Axiom qQuote
-    : let Γ := (ε ▻ ‘□’ ‘’ ‘L’) in
-      let A := (‘□’ ‘’ ‘L’)%preterm in
-      box' Γ (A ‘→’ (‘□’ ‘’ (⌜ A ⌝))).
-
-    Notation "‘‘Quote’’" := ((*box'_weaken*) qQuote) : well_typed_term_scope.
-
-    Axiom box'_weaken : let Γ := (ε ▻ ‘□’ ‘’ ‘L’) in
-                        forall {A} {H : is_closed A}, box' ε A -> box' Γ A.
-  End PostL.
-End Lob1.
-
-Module Type Lob1H (Export LC : LobContext) (Export LH : LobHypotheses LC).
-  Module Lob1' := Lob1 LC LH.
-  Declare Module Export PP : PretermPrimitives LC.
-  Declare Module Export PreL' : PreL LC PP.
-  Declare Module Export L' : Lob1'.L PP PreL'.
-  Declare Module Export PostL' : Lob1'.PostL PP PreL' L'.
-End Lob1H.
-
-Module Lob1' (LC : LobContext) (Import LH : LobHypotheses LC) (Import M : Lob1H LC LH)
-<: LobsTheorem LC LH.
-  Notation "‘‘f’’" := (box'_weaken wtt_qf) : well_typed_term_scope.
-
-  Definition lob : X.
-    refine ((fun (ℓ : □ L) => f (App (Conv2 ℓ) (Conv (Quot ℓ))))
-              (Conv2_inv
-                 (wttLambda_nd
-                    (‘□’ ‘’ ‘L’)
-                    (‘‘f’’ ‘’ ((‘‘App’’ ‘’ (qConv2 ‘‘VAR₀’’)) ‘’ ((*‘‘Conv’’ ‘’*) (‘‘Quote’’ ‘’ ‘‘VAR₀’’)))))));
-    try exact _.
-  Defined.
-End Lob1'.
-
-Module Type PretermReflectionPrimitives (Export LC : LobContext).
-  Axiom qPreterm : Preterm.
-  Notation "‘Preterm’" := qPreterm : preterm_scope.
-
-  Axiom qquote : Preterm.
-  Notation "‘quote’" := qquote : preterm_scope.
-End PretermReflectionPrimitives.
-
-Module Type TypingRules (Export LC : LobContext) (Export PP : PretermPrimitives LC).
-  Axiom capture_avoiding_subst_0 : forall (in_term : Preterm)
-                                          (new_value : Preterm),
-                                     Preterm.
-  Notation "x [ 0 ↦ y ]" := (capture_avoiding_subst_0 x y).
-  Axiom convertible : Context -> Preterm -> Preterm -> Type.
-  Axiom box'_respectful : forall {Γ A B},
-                            convertible Γ A B
-                            -> box' Γ A
-                            -> box' Γ B.
-  Axiom convertible_refl : forall {Γ}, Reflexive (convertible Γ).
-  Axiom convertible_sym : forall {Γ}, Symmetric (convertible Γ).
-  Axiom convertible_trans : forall {Γ}, Transitive (convertible Γ).
-  Axiom convertible_beta_app_lambda
-  : forall Γ A f a,
-      convertible Γ (tApp (tLambda A f) a) (capture_avoiding_subst_0 f a).
-  Axiom convertible__capture_avoiding_subst_0__tApp
-  : forall Γ A B x,
-      convertible Γ ((A ‘’ B) [ 0 ↦ x ]) ((A [ 0 ↦ x ]) ‘’ (B [ 0 ↦ x ])).
-  Axiom convertible__capture_avoiding_subst_0__qtProd
-  : forall Γ A B x,
-      convertible Γ ((A ‘‘→’’ B) [ 0 ↦ x ]) ((A [ 0 ↦ x ]) ‘‘→’’ (B [ 0 ↦ x ])).
-  Axiom convertible__capture_avoiding_subst_0__tVar0
-  : forall Γ x,
-      convertible Γ (‘VAR₀’ [ 0 ↦ x ]) x.
-
-  Axiom tProd_Proper_convertible
-  : forall Γ,
-      Proper (convertible Γ ==> eq ==> convertible Γ) tProd.
-  Existing Instance tProd_Proper_convertible.
-  Axiom qtProd_Proper_convertible
-  : forall Γ,
-      Proper (convertible Γ ==> convertible Γ ==> convertible Γ) qtProd.
-  Existing Instance qtProd_Proper_convertible.
-  Axiom tApp_Proper_convertible
-  : forall Γ,
-      Proper (convertible Γ ==> convertible Γ ==> convertible Γ) tApp.
-  Existing Instance tApp_Proper_convertible.
-  Axiom convertible__quote__qtProd
-  : forall Γ A B,
-      convertible Γ (⌜ A ‘→’ B ⌝) (⌜ A ⌝ ‘‘→’’ ⌜ B ⌝).
-  Axiom convertible__quote__closed
-  : forall Γ A x,
-      convertible Γ ((quote A) [ 0 ↦ x ]) (quote A).
-  Axiom convertible__qtApp__closed
-  : forall Γ x,
-      convertible Γ (‘App’ [ 0 ↦ x ]) (‘App’).
-  Axiom convertible__quote__app
-  : forall Γ A B,
-      convertible Γ (⌜ A ‘’ B ⌝) ((‘App’ ‘’ ⌜ A ⌝) ‘’ ⌜ B ⌝).
-End TypingRules.
-
-Module Type PretermReflectionTypingRules (Export LC : LobContext) (Export PP : PretermPrimitives LC) (Export PRP : PretermReflectionPrimitives LC) (Export TR : TypingRules LC PP).
-  Axiom convertible__qquote__closed
-  : forall Γ x,
-      convertible Γ (‘quote’ [ 0 ↦ x ]) (‘quote’).
-
-  (*Axiom box_distr_qtProd_quote
-  : forall Γ A B,
-      convertible Γ (‘□’ ‘’ (A ‘‘→’’ ⌜ B ⌝)) ((‘□’ ‘’ A) ‘‘→’’ (‘□’ ‘’ ⌜ B ⌝)).*)
-
-  Axiom box_qtProd_dom_precompose
-  : forall {Γ} A B C,
-      (box' Γ (‘□’ ‘’ B) -> box' Γ (‘□’ ‘’ A))
-      -> box' Γ (‘□’ ‘’ (A ‘‘→’’ C))
-      -> box' Γ (‘□’ ‘’ (B ‘‘→’’ C)).
-
-  (** FIXME: This seems a bit fishy... *)
-  Axiom box_quote_app_quote
-  : forall Γ T,
-      box' Γ (‘□’
-               ‘’ (‘App’ ‘’ ⌜‘□’ ⌝ ‘’ (‘App’ ‘’ ⌜T ⌝ ‘’ (‘App’ ‘’ ⌜ ‘quote’ ⌝ ‘’ ⌜ T ⌝))))
-      -> box' Γ (‘□’ ‘’ (‘App’ ‘’ ⌜‘□’ ⌝ ‘’ (‘App’ ‘’ ⌜T ⌝ ‘’ ⌜ ⌜ T ⌝ ⌝))).
-
-  Axiom box_quote_app_quote_inv
-  : forall Γ T,
-      box' Γ (‘□’ ‘’ (‘App’ ‘’ ⌜‘□’ ⌝ ‘’ (‘App’ ‘’ ⌜T ⌝ ‘’ ⌜ ⌜ T ⌝ ⌝)))
-      -> box' Γ (‘□’
-                  ‘’ (‘App’ ‘’ ⌜‘□’ ⌝ ‘’ (‘App’ ‘’ ⌜T ⌝ ‘’ (‘App’ ‘’ ⌜ ‘quote’ ⌝ ‘’ ⌜ T ⌝)))).
-End PretermReflectionTypingRules.
-
-Module Type PostL_Assumptions (LC : LobContext) (Export PP : PretermPrimitives LC) (Export PRP : PretermReflectionPrimitives LC) (Export TR : TypingRules LC PP).
-  Axiom Quot : forall T, □ T -> □ (‘□’ ‘’ ⌜ T ⌝).
-
-  Section context.
-    Context (qX qL0 : Preterm).
-    Let Γ := (ε ▻ (‘□’
-                    ‘’ (tLambda ‘Preterm’
-                                (‘App’ ‘’ ⌜ ‘□’ ⌝
-                                  ‘’ (‘App’ ‘’ ‘VAR₀’ ‘’ (‘App’ ‘’ ⌜ ‘quote’ ⌝ ‘’ ‘VAR₀’))
-                                  ‘‘→’’ ⌜ qX ⌝) ‘’ ⌜ qL0 ⌝))).
-
-    Axiom qQuote
-    : forall T,
-        let A := (‘□’ ‘’ T)%preterm in
-        box' Γ (A ‘→’ (‘□’ ‘’ (⌜ A ⌝))).
-
-    Axiom qbApp
-    : forall A' B',
-        box' Γ ((‘□’ ‘’ (A' ‘‘→’’ B')) ‘→’ (‘□’ ‘’ A') ‘→’ (‘□’ ‘’ B')).
-
-    Axiom box'_weaken
-    : forall {A} {H : is_closed A}, box' ε A -> box' Γ A.
-  End context.
-
-  Axiom App : forall {A' B'} {H : is_closed B'},
-                □ (A' ‘→’ B') -> □ A' -> □ B'.
-
-End PostL_Assumptions.
-
-Module Lob2 (LC : LobContext) (Import LH : LobHypotheses LC).
-  Module Lob1' := Lob1 LC LH.
-
-  Module L (Export PP : PretermPrimitives LC) (Export PL : PreL LC PP) (Export PRP : PretermReflectionPrimitives LC) (Export TR : TypingRules LC PP) (Export PRTR : PretermReflectionTypingRules LC PP PRP TR)
-  <: Lob1'.L PP PL.
-
-    Definition L0 (h : Preterm) : Preterm
-      := ((‘□’ ‘’ (h ‘’ (quote h))) ‘→’ ‘X’)%preterm.
-
-    Definition qL0 : Preterm
-      := tLambda
-           ‘Preterm’
-           (((‘App’ ‘’ ⌜ ‘□’ ⌝)
-               ‘’ ((‘App’ ‘’ ‘VAR₀’ ‘’ (‘App’ ‘’ ⌜ ‘quote’ ⌝ ‘’ ‘VAR₀’))))
-              ‘‘→’’
-              ⌜ ‘X’ ⌝).
-
-    Notation "‘L0’" := qL0.
-
-    Definition L : Preterm
-      := L0 ‘L0’.
-
-    Definition qL : Preterm
-      := ‘L0’ ‘’ ⌜ ‘L0’ ⌝.
-
-    Notation "‘L’" := qL.
-  End L.
-
-  Module PostL (Export PP : PretermPrimitives LC) (Export PL : PreL LC PP) (Export PRP : PretermReflectionPrimitives LC) (Export TR : TypingRules LC PP) (Export PRTR : PretermReflectionTypingRules LC PP PRP TR) (LA : PostL_Assumptions LC PP PRP TR).
-    Module L' := L PP PL PRP TR PRTR.
-    Include L'.
-
-    Module M <: Lob1'.PostL PP PL L'.
-
-      Hint Rewrite convertible__qtApp__closed convertible__capture_avoiding_subst_0__tApp convertible__quote__closed convertible__quote__app convertible__capture_avoiding_subst_0__tVar0 convertible__qquote__closed convertible__capture_avoiding_subst_0__qtProd convertible__quote__qtProd convertible_beta_app_lambda : convdb.
-
-      Local Ltac set_evars :=
-        repeat match goal with
-                 | [ |- appcontext[?E] ] => is_evar E; let e := fresh in set (e := E)
-               end.
-
-      Local Ltac subst_body :=
-        repeat match goal with
-                 | [ H := _ |- _ ] => subst H
-               end.
-
-      Local Ltac conv_rewrite
-        := set_evars;
-          repeat match goal with
-                   | [ |- convertible _ ?x ?x ] => reflexivity
-                   | [ |- convertible _ (?x ‘’ _) (?x ‘’ _) ]
-                     => apply tApp_Proper_convertible; [ reflexivity | ]
-                   | [ |- convertible _ (_ ‘‘→’’ _) (_ ‘‘→’’ _) ]
-                     => apply qtProd_Proper_convertible
-                   | [ |- convertible _ (_ ‘→’ ?x) _ ]
-                     => apply tProd_Proper_convertible; [ | reflexivity ]
-                   | _ => progress rewrite_strat repeat (topdown repeat (hints convdb))
-                 (*| _ => progress rewrite ?convertible__capture_avoiding_subst_0__tApp, ?convertible__qtApp__closed, ?convertible__quote__closed, ?convertible__quote__app, ?convertible__capture_avoiding_subst_0__tVar0, ?convertible__qquote__closed, ?convertible__capture_avoiding_subst_0__qtProd, ?convertible__quote__qtProd, ?convertible_beta_app_lambda*)
-                 end;
-          subst_body.
-
-
-
-      Definition Conv : □ (‘□’ ‘’ ⌜ L ⌝) -> □ (‘□’ ‘’ ‘L’).
-      Proof.
-        unfold box, L, qL.
-        do_shelve
-          ltac:(refine (fun box_L => let box_L' := box'_respectful _ box_L in _ box_L')).
-        { unfold L0, qL0; conv_rewrite.
-          reflexivity. }
-        { clear.
-          unfold L0, qL0.
-          intro box_L.
-          eapply box'_respectful.
-          { conv_rewrite.
-            reflexivity. }
-          { revert box_L.
-            match goal with
-              | [ |- context[quote (quote ?X)] ] => generalize X; intro T
-            end.
-            apply box_qtProd_dom_precompose.
-            apply box_quote_app_quote. } }
-      Defined.
-
-      Definition Conv2 : □ L -> □ (‘□’ ‘’ ‘L’ ‘→’ ‘X’)
-        := fun x => x.
-      Definition Conv2_inv : □ (‘□’ ‘’ ‘L’ ‘→’ ‘X’) -> □ L
-        := fun x => x.
-      Definition qConv2 (Γ := (ε ▻ ‘□’ ‘’ ‘L’))
-      : box' Γ (‘□’ ‘’ ‘L’) -> box' Γ (‘□’ ‘’ (⌜‘□’ ‘’ ‘L’ ⌝ ‘‘→’’ ⌜ ‘X’ ⌝)).
-      Proof.
-        unfold qL.
-        do_shelve
-          ltac:(refine (fun box_L => let box_L' := box'_respectful _ box_L in _ box_L')).
-        { unfold L0, qL0; conv_rewrite.
-          reflexivity. }
-        { clear.
-          unfold L0, qL0.
-          intro box_L.
-          eapply box'_respectful.
-          { conv_rewrite.
-            reflexivity. }
-          { revert box_L.
-            match goal with
-              | [ |- context[quote (quote ?X)] ] => generalize X; intro T
-            end.
-            apply box_qtProd_dom_precompose.
-            apply box_quote_app_quote_inv. } }
-      Defined.
-
-      (*Axiom qConv
-  : □ (‘□’ ‘’ ⌜‘□’ ‘’ ⌜L ⌝ ⌝ ‘→’ ‘□’ ‘’ ⌜ ‘□’ ‘’ ‘L’ ⌝).
-
-  Notation "‘‘Conv’’" := (box'_weaken qConv) : well_typed_term_scope.*)
-
-      Definition Quot : □ L -> □ (‘□’ ‘’ ⌜ L ⌝)
-        := LA.Quot _.
-
-      Global Instance convertible_Proper_flip_arrow {Γ}
-      : Proper (convertible Γ ==> convertible Γ ==> flip arrow) (convertible Γ).
-      Proof.
-        intros ?? H ?? H' H''.
-        rewrite H, H''.
-        rewrite <- H'.
-        reflexivity.
-      Qed.
-
-      Definition qbApp
-      : let Γ := (ε ▻ ‘□’ ‘’ ‘L’) in
-        forall (A' := (⌜‘□’ ‘’ ‘L’ ⌝)%preterm)
-               (B' := (⌜‘X’ ⌝)%preterm),
-          box' Γ ((‘□’ ‘’ (A' ‘‘→’’ B')) ‘→’ (‘□’ ‘’ A') ‘→’ (‘□’ ‘’ B'))
-        := LA.qbApp _ _ _ _.
-
-      Notation "‘‘App’’" := ((*box'_weaken*) qbApp) : well_typed_term_scope.
-
-      Definition qQuote
-      : let Γ := ε ▻ ‘□’ ‘’ ‘L’ in
-        let A := (‘□’ ‘’ ‘L’)%preterm in
-        box' Γ (A ‘→’ (‘□’ ‘’ (⌜ A ⌝)))
-        := LA.qQuote _ _ _.
-
-      Notation "‘‘Quote’’" := ((*box'_weaken*) qQuote) : well_typed_term_scope.
-
-      Definition App : (let A' := ‘□’ ‘’ ‘L’ in
-                        let B' := ‘X’ in
-                        □ (A' ‘→’ B') -> □ A' -> □ B')
-        := (@LA.App _ _ LH.qX_closed).
-
-      Definition box'_weaken : let Γ := (ε ▻ ‘□’ ‘’ ‘L’) in
-                               forall {A} {H : is_closed A}, box' ε A -> box' Γ A
-        := @LA.box'_weaken _ _.
-
-    End M.
-  End PostL.
-End Lob2.
-
-Module Type Lob2H (Export LC : LobContext) (Export LH : LobHypotheses LC).
-  Module Lob2' := Lob2 LC LH.
-  Declare Module Export PP : PretermPrimitives LC.
-  Declare Module Export PreL' : PreL LC PP.
-  Declare Module Export PRP : PretermReflectionPrimitives LC.
-  Declare Module Export TR : TypingRules LC PP.
-  Declare Module Export PRTR : PretermReflectionTypingRules LC PP PRP TR.
-  Declare Module Export LA : PostL_Assumptions LC PP PRP TR.
-End Lob2H.
-
-Module Lob2'0 (LC : LobContext) (LH : LobHypotheses LC) (M : Lob2H LC LH)
-<: LobsTheorem LC LH.
-  Module Lob1HV <: Lob1H LC LH.
-    Include M.
-    Include M.Lob2'.
-    Module L' <: Lob1'.L PP PreL'
-      := L PP PreL' PRP TR PRTR.
-    Module PostL'' := M.Lob2'.PostL PP PreL' PRP TR PRTR LA.
-    Module PostL' <: Lob1'.PostL PP PreL' L'
-      := PostL''.M.
-  End Lob1HV.
-  Module M' := Lob1' LC LH Lob1HV.
-  Definition lob := M'.lob.
-End Lob2'0.
-
-Module LobOfPreLob
-       (Export LC : LobContext)
-       (Export LH : LobHypotheses LC)
-       (Export PP : PretermPrimitives LC)
-       (Export PreL' : PreL LC PP)
-       (Export PRP : PretermReflectionPrimitives LC)
-       (Export TR : TypingRules LC PP)
-       (Export PRTR : PretermReflectionTypingRules LC PP PRP TR)
-       (Export LA : PostL_Assumptions LC PP PRP TR)
-<: LobsTheorem LC LH.
-  Module M'0 <: Lob2H LC LH.
-    Module Lob2' := Lob2 LC LH.
-    Module PP := PP.
-    Module PreL' := PreL'.
-    Module PRP := PRP.
-    Module TR := TR.
-    Module PRTR := PRTR.
-    Module LA := LA.
-  End M'0.
-  Include (Lob2'0 LC LH M'0).
-End LobOfPreLob.
+  Module TQ' := TQ LC LH TP QP.
+  Include (Lob0 LC LH TP QP TQ').
+End Lob.
